

$$Ex 1: K_{t+1} = (1-\delta)K_t + \underline{I_t} = F(K_t, I_t)$$

$$LL: \hat{K}_{t+1} = \frac{F_K(K, I)K}{F(K, I)} \hat{K}_t + \frac{F_I(K, I)\underline{I}}{F(K, I)} \hat{I}_t$$

$$= \frac{(1-\delta)K}{K} \hat{K}_t + \frac{1 \times \delta K}{K} \hat{I}_t$$

$$= (1-\delta) \hat{K}_t + \delta \hat{I}_t$$

Ex 2:  $Y_t = C_t + I_t = F(C_t, I_t)$

LL:  $\hat{Y}_t = \frac{F_C(C, I) C}{F(C, I)} \hat{C}_t + \frac{F_I(C, I) I}{F(C, I)} \hat{I}_t$

$$= \frac{C}{Y} \tilde{C}_t + \frac{I}{Y} \hat{I}_t$$



$$\underbrace{\frac{1}{C_t}}_{G(C_t)} = \underbrace{\beta E_t \left[ (R^r_{t+1} + (1-\delta)) \frac{1}{C_{t+1}} \right]}_{H(R^r_{t+1}, C_{t+1})}$$

$$\text{RHS: } \frac{G_C(C) C}{G(C)} \hat{C}_{t+1} = \frac{-\frac{1}{C^2} C}{\frac{1}{C}} \hat{C}_t = -\hat{C}_t$$

$$\begin{aligned} \text{LHS: } & \frac{H_R(R^r, C) R^r}{H(R^r, C)} E_t \hat{r}_{t+1}^r + \frac{H_C(R^r, C) C}{H(R^r, C)} E_t \hat{C}_{t+1} \\ &= \frac{\beta \frac{1}{C} R^r}{\frac{1}{C}} E_t \hat{r}_{t+1}^r + \frac{\beta (R^r + (1-\delta)) (-\frac{1}{C^2}) C}{\frac{1}{C}} E_t \hat{C}_{t+1} \end{aligned}$$

$$= \beta R^r E_t \hat{r}_{t+1}^r - E_t \hat{C}_{t+1}$$

$$\Rightarrow \hat{C}_{t+1} = -\beta R^r E_t \hat{r}_{t+1}^r + E_t \hat{C}_{t+1}$$